@prefix :        <http://w3id.org/dpp#> .
@prefix dpp:     <http://w3id.org/dpp#> .
@prefix owl:     <http://www.w3.org/2002/07/owl#> .
@prefix rdf:     <http://www.w3.org/1999/02/22-rdf-syntax-ns#> .
@prefix rdfs:    <http://www.w3.org/2000/01/rdf-schema#> .
@prefix xsd:     <http://www.w3.org/2001/XMLSchema#> .
@prefix dcterms: <http://purl.org/dc/terms/> .

@base <http://w3id.org/dpp#> .

<https://w3id.org/dpp/useandmaintenance>
    a owl:Ontology ;
    owl:versionIRI   <https://w3id.org/dpp/useandmaintenance/1.0> ;
    owl:versionInfo  "1.0" ;
    dcterms:title    "Digital Product Passport â€“ Use and Maintenance Module Ontology"@en ;
    dcterms:creator  "Rahel Kebede" ;
    dcterms:contributor "Peter Johansson" , "Annika Moscati" ;
    dcterms:description
        "This ontology defines concepts and properties related to the use phase and maintenance of products within a Digital Product Passport (DPP), covering usage instructions, maintenance schedules, and operational performance data."@en ;
    dcterms:created  "2024-01-10"^^xsd:date ;
    dcterms:license  <https://creativecommons.org/licenses/by/4.0/> ;
    owl:imports      <https://w3id.org/dpp> .

#################################################################
#    Annotation properties
#################################################################

###  http://ontologydesignpatterns.org/opla#isNativeTo
<http://ontologydesignpatterns.org/opla#isNativeTo> rdf:type owl:AnnotationProperty .


###  http://ontologydesignpatterns.org/opla#reusesPatternAsTemplate
<http://ontologydesignpatterns.org/opla#reusesPatternAsTemplate> rdf:type owl:AnnotationProperty .


###  http://ontologydesignpatterns.org/opla-sd#entityPosition
<http://ontologydesignpatterns.org/opla-sd#entityPosition> rdf:type owl:AnnotationProperty ;
                                                           <http://ontologydesignpatterns.org/opla#isNativeTo> <http://www.w3id.org/dpp/UseAndMaintenance-modules/e69a1c0c-bdf8-472b-8b5f-6cf8952bd8df> ,
                                                                                                               <http://www.w3id.org/dpp/UseAndMaintenance-modules/f5199444-758a-40b7-ad67-4a2a99ee3d2c> ,
                                                                                                               <http://www.w3id.org/dpp/UseAndMaintenance-modules/35950a21-8fcd-4fbd-a876-e4ec20d5007c> ,
                                                                                                               <http://www.w3id.org/dpp/UseAndMaintenance-modules/3688421d-d7b1-45c5-b117-5cfe3320ffd4> ,
                                                                                                               <http://www.w3id.org/dpp/UseAndMaintenance-modules/9892962b-836d-4b8e-b823-bfbc6d2d1e7b> .


###  http://ontologydesignpatterns.org/opla-sd#entityPositionX
<http://ontologydesignpatterns.org/opla-sd#entityPositionX> rdf:type owl:AnnotationProperty ;
                                                            <http://ontologydesignpatterns.org/opla#isNativeTo> <http://www.w3id.org/dpp/UseAndMaintenance-modules/e69a1c0c-bdf8-472b-8b5f-6cf8952bd8df> ,
                                                                                                                <http://www.w3id.org/dpp/UseAndMaintenance-modules/f5199444-758a-40b7-ad67-4a2a99ee3d2c> ,
                                                                                                                <http://www.w3id.org/dpp/UseAndMaintenance-modules/35950a21-8fcd-4fbd-a876-e4ec20d5007c> ,
                                                                                                                <http://www.w3id.org/dpp/UseAndMaintenance-modules/3688421d-d7b1-45c5-b117-5cfe3320ffd4> ,
                                                                                                                <http://www.w3id.org/dpp/UseAndMaintenance-modules/9892962b-836d-4b8e-b823-bfbc6d2d1e7b> .


###  http://ontologydesignpatterns.org/opla-sd#entityPositionY
<http://ontologydesignpatterns.org/opla-sd#entityPositionY> rdf:type owl:AnnotationProperty ;
                                                            <http://ontologydesignpatterns.org/opla#isNativeTo> <http://www.w3id.org/dpp/UseAndMaintenance-modules/e69a1c0c-bdf8-472b-8b5f-6cf8952bd8df> ,
                                                                                                                <http://www.w3id.org/dpp/UseAndMaintenance-modules/f5199444-758a-40b7-ad67-4a2a99ee3d2c> ,
                                                                                                                <http://www.w3id.org/dpp/UseAndMaintenance-modules/35950a21-8fcd-4fbd-a876-e4ec20d5007c> ,
                                                                                                                <http://www.w3id.org/dpp/UseAndMaintenance-modules/3688421d-d7b1-45c5-b117-5cfe3320ffd4> ,
                                                                                                                <http://www.w3id.org/dpp/UseAndMaintenance-modules/9892962b-836d-4b8e-b823-bfbc6d2d1e7b> .


#################################################################
#    Object Properties
#################################################################

###  http://www.w3id.org/dpp#hasActivity
dpp:hasActivity rdf:type owl:ObjectProperty ;
                rdfs:domain dpp:MaintenanceTask ;
                rdfs:range dpp:Activity ;
                rdfs:comment "Links the maintenance task to the activities involved in it"@en ;
                rdfs:label "hasActivity"@en .


###  http://www.w3id.org/dpp#hasCleaningInstruction
dpp:hasCleaningInstruction rdf:type owl:ObjectProperty ;
                           rdfs:domain dpp:MaintenanceTask ;
                           rdfs:range dpp:Cleaning ;
                           rdfs:comment "Links the maintenance task to its cleaning instructions"@en ;
                           rdfs:label "hasCleaningInstruction"@en .


###  http://www.w3id.org/dpp#hasFailureData
dpp:hasFailureData rdf:type owl:ObjectProperty ;
                   rdfs:domain dpp:Product ;
                   rdfs:range dpp:FailureData ;
                   rdfs:comment "Links the product to its failure data, including mean time between failures"@en ;
                   rdfs:label "hasFailureData"@en .


###  http://www.w3id.org/dpp#hasMaintenanceRecord
dpp:hasMaintenanceRecord rdf:type owl:ObjectProperty ;
                         rdfs:domain dpp:MaintenanceTask ;
                         rdfs:range dpp:MaintenanceRecord ;
                         rdfs:comment "Links the maintenance task to its maintenance records"@en ;
                         rdfs:label "hasMaintenanceRecord"@en .


###  http://www.w3id.org/dpp#hasManual
dpp:hasManual rdf:type owl:ObjectProperty ;
              rdfs:domain dpp:Product ;
              rdfs:range dpp:Manual ;
              rdfs:comment "Links the product to its user manual, warnings, or safety information"@en ;
              rdfs:label "hasManual"@en .


###  http://www.w3id.org/dpp#hasOwnershipStatus
dpp:hasOwnershipStatus rdf:type owl:ObjectProperty ;
                       rdfs:domain dpp:Product ;
                       rdfs:range dpp:OwnershipStatus ;
                       rdfs:comment "Links the product to its ownership status"@en ;
                       rdfs:label "hasOwnershipStatus"@en .


###  http://www.w3id.org/dpp#hasRealUseInformation
dpp:hasRealUseInformation rdf:type owl:ObjectProperty ;
                          rdfs:domain dpp:Product ;
                          rdfs:range dpp:RealUseInformation ;
                          rdfs:comment "Links the product to its real use information"@en ;
                          rdfs:label "hasRealUseInformation"@en .


###  http://www.w3id.org/dpp#hasServiceHistory
dpp:hasServiceHistory rdf:type owl:ObjectProperty ;
                      rdfs:domain dpp:Product ;
                      rdfs:range dpp:ServiceHistory ;
                      rdfs:comment "Links the product to its service history"@en ;
                      rdfs:label "hasServiceHistory"@en .


###  http://www.w3id.org/dpp#hasUpdate
dpp:hasUpdate rdf:type owl:ObjectProperty ;
              rdfs:domain dpp:Product ;
              rdfs:range dpp:Update ;
              rdfs:comment "Links the product to its updates during operations"@en ;
              rdfs:label "hasUpdate"@en .


###  http://www.w3id.org/dpp#hasUseCondition
dpp:hasUseCondition rdf:type owl:ObjectProperty ;
                    rdfs:domain dpp:Product ;
                    rdfs:range dpp:UseCondition ;
                    rdfs:comment "Links the product to the conditions under which it should be used"@en ;
                    rdfs:label "hasUseCondition"@en .


###  http://www.w3id.org/dpp#hasVerification
dpp:hasVerification rdf:type owl:ObjectProperty ;
                    rdfs:domain dpp:Product ;
                    rdfs:range dpp:Verification ;
                    rdfs:comment "Links the product to its verification data"@en ;
                    rdfs:label "hasVerification"@en .


###  http://www.w3id.org/dpp#locatedIn
dpp:locatedIn rdf:type owl:ObjectProperty ;
              rdfs:domain dpp:Product ;
              rdfs:range dpp:Building ;
              rdfs:comment "The building where the product is located"@en ;
              rdfs:label "locatedIn"@en .


###  http://www.w3id.org/dpp#requiresConsumable
dpp:requiresConsumable rdf:type owl:ObjectProperty ;
                       rdfs:domain dpp:Product ;
                       rdfs:range dpp:Consumable ;
                       rdfs:comment "Links the product to the consumables it requires"@en ;
                       rdfs:label "requiresConsumable"@en .


###  http://www.w3id.org/dpp#requiresMaintenance
dpp:requiresMaintenance rdf:type owl:ObjectProperty ;
                        rdfs:domain dpp:Product ;
                        rdfs:range dpp:MaintenanceTask ;
                        rdfs:comment "A property that links a Product to the MaintenanceTask(s) it requires"@en ;
                        rdfs:label "requiresMaintenance"@en .


###  http://www.w3id.org/dpp#usesProduct
dpp:usesProduct rdf:type owl:ObjectProperty ;
                rdfs:domain dpp:User ;
                rdfs:range dpp:Product ;
                rdfs:comment "Links the user to the products they use"@en ;
                rdfs:label "usesProduct"@en .


###  http://www.w3id.org/dpp/UseAndMaintenance#attributedTo
:attributedTo rdf:type owl:ObjectProperty ;
              rdfs:domain :EntityWithProvenance ;
              rdfs:range :Agent ;
              <http://ontologydesignpatterns.org/opla#isNativeTo> <http://www.w3id.org/dpp/UseAndMaintenance-modules/9892962b-836d-4b8e-b823-bfbc6d2d1e7b> .


###  http://www.w3id.org/dpp/UseAndMaintenance#contains
:contains rdf:type owl:ObjectProperty ;
          rdfs:domain :TemporalExtent ;
          rdfs:range :ComplexTemporalExtent ;
          <http://ontologydesignpatterns.org/opla#isNativeTo> <http://www.w3id.org/dpp/UseAndMaintenance-modules/35950a21-8fcd-4fbd-a876-e4ec20d5007c> .


###  http://www.w3id.org/dpp/UseAndMaintenance#coveredBy
:coveredBy rdf:type owl:ObjectProperty ;
           rdfs:domain dpp:Product ;
           rdfs:range :Warranty .


###  http://www.w3id.org/dpp/UseAndMaintenance#derivedFrom
:derivedFrom rdf:type owl:ObjectProperty ;
             rdfs:domain :EntityWithProvenance ;
             rdfs:range :EntityWithProvenance ;
             <http://ontologydesignpatterns.org/opla#isNativeTo> <http://www.w3id.org/dpp/UseAndMaintenance-modules/9892962b-836d-4b8e-b823-bfbc6d2d1e7b> .


###  http://www.w3id.org/dpp/UseAndMaintenance#endsAt
:endsAt rdf:type owl:ObjectProperty ;
        rdfs:domain :TimeInterval ;
        rdfs:range :PointInTime ;
        <http://ontologydesignpatterns.org/opla#isNativeTo> <http://www.w3id.org/dpp/UseAndMaintenance-modules/35950a21-8fcd-4fbd-a876-e4ec20d5007c> .


###  http://www.w3id.org/dpp/UseAndMaintenance#followsSchedule
:followsSchedule rdf:type owl:ObjectProperty ;
                 rdfs:domain dpp:MaintenanceTask ;
                 rdfs:range :MaintenanceSchedule .


###  http://www.w3id.org/dpp/UseAndMaintenance#generatedBy
:generatedBy rdf:type owl:ObjectProperty ;
             rdfs:domain :EntityWithProvenance ;
             rdfs:range :ProvenanceActivity ;
             <http://ontologydesignpatterns.org/opla#isNativeTo> <http://www.w3id.org/dpp/UseAndMaintenance-modules/9892962b-836d-4b8e-b823-bfbc6d2d1e7b> .


###  http://www.w3id.org/dpp/UseAndMaintenance#hasConsumableQuantity
:hasConsumableQuantity rdf:type owl:ObjectProperty ;
                       rdfs:subPropertyOf :hasQuantity ;
                       rdfs:domain dpp:Consumable ;
                       rdfs:range :Quantity .


###  http://www.w3id.org/dpp/UseAndMaintenance#hasContactInformation
:hasContactInformation rdf:type owl:ObjectProperty ;
                       rdfs:domain dpp:User ,
                                   [ rdf:type owl:Class ;
                                     owl:unionOf ( dpp:User
                                                   :Warranty
                                                 )
                                   ] ;
                       rdfs:range :ContactInformation .


###  http://www.w3id.org/dpp/UseAndMaintenance#hasCostQuantityKind
:hasCostQuantityKind rdf:type owl:ObjectProperty ;
                     rdfs:subPropertyOf :hasQuantityKind ;
                     rdfs:domain :CostQuantity ;
                     rdfs:range :MaintenanceCost .


###  http://www.w3id.org/dpp/UseAndMaintenance#hasLifespanQuantity
:hasLifespanQuantity rdf:type owl:ObjectProperty ;
                     rdfs:subPropertyOf :hasQuantity ;
                     rdfs:domain dpp:Product ;
                     rdfs:range :LifespanQuantity .


###  http://www.w3id.org/dpp/UseAndMaintenance#hasMaintenanceCost
:hasMaintenanceCost rdf:type owl:ObjectProperty ;
                    rdfs:domain dpp:MaintenanceTask ;
                    rdfs:range :CostQuantity .


###  http://www.w3id.org/dpp/UseAndMaintenance#hasQualityLossQuantity
:hasQualityLossQuantity rdf:type owl:ObjectProperty ;
                        rdfs:subPropertyOf :hasQuantity ;
                        rdfs:domain dpp:Product ;
                        rdfs:range :QualityLossQuantity .


###  http://www.w3id.org/dpp/UseAndMaintenance#hasQuantity
:hasQuantity rdf:type owl:ObjectProperty ;
             rdfs:domain dpp:MaintenanceTask ;
             rdfs:range :Quantity .


###  http://www.w3id.org/dpp/UseAndMaintenance#hasQuantityKind
:hasQuantityKind rdf:type owl:ObjectProperty ;
                 rdfs:domain :Quantity ;
                 rdfs:range :QuantityKind ;
                 <http://ontologydesignpatterns.org/opla#isNativeTo> <http://www.w3id.org/dpp/UseAndMaintenance-modules/3688421d-d7b1-45c5-b117-5cfe3320ffd4> .


###  http://www.w3id.org/dpp/UseAndMaintenance#hasQuantityValue
:hasQuantityValue rdf:type owl:ObjectProperty ;
                  rdfs:domain :Quantity ;
                  rdfs:range :QuantityValue ;
                  <http://ontologydesignpatterns.org/opla#isNativeTo> <http://www.w3id.org/dpp/UseAndMaintenance-modules/3688421d-d7b1-45c5-b117-5cfe3320ffd4> .


###  http://www.w3id.org/dpp/UseAndMaintenance#hasReferenceSystem
:hasReferenceSystem rdf:type owl:ObjectProperty ;
                    rdfs:domain :PointInTime ;
                    rdfs:range :ReferenceSystem ;
                    <http://ontologydesignpatterns.org/opla#isNativeTo> <http://www.w3id.org/dpp/UseAndMaintenance-modules/35950a21-8fcd-4fbd-a876-e4ec20d5007c> .


###  http://www.w3id.org/dpp/UseAndMaintenance#hasSafetyMeasure
:hasSafetyMeasure rdf:type owl:ObjectProperty ;
                  rdfs:domain dpp:MaintenanceTask ;
                  rdfs:range :SafetyMeasure ;
                  rdfs:label "hasSafetyMeasure" .


###  http://www.w3id.org/dpp/UseAndMaintenance#hasTemporalExtent
:hasTemporalExtent rdf:type owl:ObjectProperty ;
                   rdfs:domain :AgentRole ;
                   rdfs:range :TemporalExtent ;
                   <http://ontologydesignpatterns.org/opla#isNativeTo> <http://www.w3id.org/dpp/UseAndMaintenance-modules/f5199444-758a-40b7-ad67-4a2a99ee3d2c> .


###  http://www.w3id.org/dpp/UseAndMaintenance#hasUnit
:hasUnit rdf:type owl:ObjectProperty ;
         rdfs:domain :QuantityValue ;
         rdfs:range :Unit ;
         <http://ontologydesignpatterns.org/opla#isNativeTo> <http://www.w3id.org/dpp/UseAndMaintenance-modules/3688421d-d7b1-45c5-b117-5cfe3320ffd4> .


###  http://www.w3id.org/dpp/UseAndMaintenance#hasValue
:hasValue rdf:type owl:ObjectProperty ;
          rdfs:domain :PointInTime ;
          rdfs:range :Value ;
          <http://ontologydesignpatterns.org/opla#isNativeTo> <http://www.w3id.org/dpp/UseAndMaintenance-modules/35950a21-8fcd-4fbd-a876-e4ec20d5007c> .


###  http://www.w3id.org/dpp/UseAndMaintenance#performedBy
:performedBy rdf:type owl:ObjectProperty ;
             rdfs:domain :ProvenanceActivity ;
             rdfs:range :Agent ;
             <http://ontologydesignpatterns.org/opla#isNativeTo> <http://www.w3id.org/dpp/UseAndMaintenance-modules/9892962b-836d-4b8e-b823-bfbc6d2d1e7b> .


###  http://www.w3id.org/dpp/UseAndMaintenance#performsAgentRole
:performsAgentRole rdf:type owl:ObjectProperty ;
                   rdfs:domain :Agent ;
                   rdfs:range :AgentRole ;
                   <http://ontologydesignpatterns.org/opla#isNativeTo> <http://www.w3id.org/dpp/UseAndMaintenance-modules/f5199444-758a-40b7-ad67-4a2a99ee3d2c> .


###  http://www.w3id.org/dpp/UseAndMaintenance#providesAgentRole
:providesAgentRole rdf:type owl:ObjectProperty ;
                   rdfs:domain dpp:MaintenanceTask ;
                   rdfs:range :AgentRole ;
                   <http://ontologydesignpatterns.org/opla#isNativeTo> <http://www.w3id.org/dpp/UseAndMaintenance-modules/f5199444-758a-40b7-ad67-4a2a99ee3d2c> .


###  http://www.w3id.org/dpp/UseAndMaintenance#startsFrom
:startsFrom rdf:type owl:ObjectProperty ;
            rdfs:domain :TimeInterval ;
            rdfs:range :PointInTime ;
            <http://ontologydesignpatterns.org/opla#isNativeTo> <http://www.w3id.org/dpp/UseAndMaintenance-modules/35950a21-8fcd-4fbd-a876-e4ec20d5007c> .


###  http://www.w3id.org/dpp/UseAndMaintenance#targetUser
:targetUser rdf:type owl:ObjectProperty ;
            rdfs:domain :IntendedUse ;
            rdfs:range dpp:User ;
            rdfs:comment "it references a class of users for whom the product is intended" .


#################################################################
#    Data properties
#################################################################

###  http://www.w3id.org/dpp#availability
dpp:availability rdf:type owl:DatatypeProperty ;
                 rdfs:domain dpp:Consumable ;
                 rdfs:range xsd:string ;
                 <http://ontologydesignpatterns.org/opla-sd#entityPosition> [ <http://ontologydesignpatterns.org/opla-sd#entityPositionX> "-170.19696251869073"^^xsd:double ;
                                                                              <http://ontologydesignpatterns.org/opla-sd#entityPositionY> "509.74413946338626"^^xsd:double ;
                                                                              rdfs:comment "This is an entity positioning annotation generated by CoModIDE (https://comodide.com/). Removing this annotation will break rendering the CoModIDE schema diagram view."@en
                                                                            ] ;
                 rdfs:comment "The availability status of the consumable"@en ;
                 rdfs:label "availability"@en .


###  http://www.w3id.org/dpp#lifeSpan
dpp:lifeSpan rdf:type owl:DatatypeProperty ;
             rdfs:domain dpp:Product ;
             rdfs:range xsd:integer ;
             <http://ontologydesignpatterns.org/opla-sd#entityPosition> [ <http://ontologydesignpatterns.org/opla-sd#entityPositionX> "290.16435007053667"^^xsd:double ;
                                                                          <http://ontologydesignpatterns.org/opla-sd#entityPositionY> "1079.697636947784"^^xsd:double ;
                                                                          rdfs:comment "This is an entity positioning annotation generated by CoModIDE (https://comodide.com/). Removing this annotation will break rendering the CoModIDE schema diagram view."@en
                                                                        ] ;
             rdfs:comment "The expected life span of the product or material"@en ;
             rdfs:label "lifeSpan"@en .


###  http://www.w3id.org/dpp#maintenanceInstructions
dpp:maintenanceInstructions rdf:type owl:DatatypeProperty ;
                            rdfs:domain dpp:MaintenanceTask ;
                            rdfs:range xsd:string ;
                            <http://ontologydesignpatterns.org/opla-sd#entityPosition> [ <http://ontologydesignpatterns.org/opla-sd#entityPositionX> "50.072629397576094"^^xsd:double ;
                                                                                         <http://ontologydesignpatterns.org/opla-sd#entityPositionY> "-279.991802785798"^^xsd:double ;
                                                                                         rdfs:comment "This is an entity positioning annotation generated by CoModIDE (https://comodide.com/). Removing this annotation will break rendering the CoModIDE schema diagram view."@en
                                                                                       ] ;
                            rdfs:comment "Detailed instructions on how to perform the maintenance task"@en ;
                            rdfs:label "maintenanceInstructions"@en .


###  http://www.w3id.org/dpp#qualityLossOverTime
dpp:qualityLossOverTime rdf:type owl:DatatypeProperty ;
                        rdfs:domain dpp:Product ;
                        rdfs:range xsd:float ;
                        <http://ontologydesignpatterns.org/opla-sd#entityPosition> [ <http://ontologydesignpatterns.org/opla-sd#entityPositionX> "-210.25670602428727"^^xsd:double ;
                                                                                     <http://ontologydesignpatterns.org/opla-sd#entityPositionY> "740.2806459768744"^^xsd:double ;
                                                                                     rdfs:comment "This is an entity positioning annotation generated by CoModIDE (https://comodide.com/). Removing this annotation will break rendering the CoModIDE schema diagram view."@en
                                                                                   ] ;
                        rdfs:comment "Consideration of the loss of quality of the product over time"@en ;
                        rdfs:label "qualityLossOvertime"@en .


###  http://www.w3id.org/dpp#taskDescription
dpp:taskDescription rdf:type owl:DatatypeProperty ;
                    rdfs:domain dpp:MaintenanceTask ;
                    rdfs:range xsd:string ;
                    <http://ontologydesignpatterns.org/opla-sd#entityPosition> [ <http://ontologydesignpatterns.org/opla-sd#entityPositionX> "430.3142670299586"^^xsd:double ;
                                                                                 <http://ontologydesignpatterns.org/opla-sd#entityPositionY> "-429.8284968629161"^^xsd:double ;
                                                                                 rdfs:comment "This is an entity positioning annotation generated by CoModIDE (https://comodide.com/). Removing this annotation will break rendering the CoModIDE schema diagram view."@en
                                                                               ] ;
                    rdfs:comment "A brief description of the maintenance task"@en ;
                    rdfs:label "taskDescription"@en .


###  http://www.w3id.org/dpp#taskFrequency
dpp:taskFrequency rdf:type owl:DatatypeProperty ;
                  rdfs:domain dpp:MaintenanceTask ;
                  rdfs:range xsd:integer ;
                  <http://ontologydesignpatterns.org/opla-sd#entityPosition> [ <http://ontologydesignpatterns.org/opla-sd#entityPositionX> "590.1807497425808"^^xsd:double ;
                                                                               <http://ontologydesignpatterns.org/opla-sd#entityPositionY> "-389.54463669251703"^^xsd:double ;
                                                                               rdfs:comment "This is an entity positioning annotation generated by CoModIDE (https://comodide.com/). Removing this annotation will break rendering the CoModIDE schema diagram view."@en
                                                                             ] ;
                  rdfs:comment "The frequency at which the maintenance task should be performed, e.g., daily, monthly, or after a specific number of operating hours"@en ;
                  rdfs:label "taskFrequency"@en .


###  http://www.w3id.org/dpp/UseAndMaintenance#activityName
:activityName rdf:type owl:DatatypeProperty ;
              rdfs:domain dpp:Activity ;
              rdfs:range xsd:Name ;
              <http://ontologydesignpatterns.org/opla-sd#entityPosition> [ <http://ontologydesignpatterns.org/opla-sd#entityPositionX> "590.4451365399727"^^xsd:double ;
                                                                           <http://ontologydesignpatterns.org/opla-sd#entityPositionY> "509.5636058256862"^^xsd:double ;
                                                                           rdfs:comment "This is an entity positioning annotation generated by CoModIDE (https://comodide.com/). Removing this annotation will break rendering the CoModIDE schema diagram view."@en
                                                                         ] ;
              rdfs:label "activityName" .


###  http://www.w3id.org/dpp/UseAndMaintenance#coverageDetails
:coverageDetails rdf:type owl:DatatypeProperty ;
                 rdfs:domain :Warranty ;
                 rdfs:range xsd:string ;
                 <http://ontologydesignpatterns.org/opla-sd#entityPosition> [ <http://ontologydesignpatterns.org/opla-sd#entityPositionX> "809.9731528527384"^^xsd:double ;
                                                                              <http://ontologydesignpatterns.org/opla-sd#entityPositionY> "659.8177395654905"^^xsd:double ;
                                                                              rdfs:comment "This is an entity positioning annotation generated by CoModIDE (https://comodide.com/). Removing this annotation will break rendering the CoModIDE schema diagram view."@en
                                                                            ] .


###  http://www.w3id.org/dpp/UseAndMaintenance#hasNumericValue
:hasNumericValue rdf:type owl:DatatypeProperty ;
                 rdfs:domain :QuantityValue ;
                 rdfs:range xsd:double ;
                 <http://ontologydesignpatterns.org/opla#isNativeTo> <http://www.w3id.org/dpp/UseAndMaintenance-modules/3688421d-d7b1-45c5-b117-5cfe3320ffd4> ;
                 <http://ontologydesignpatterns.org/opla-sd#entityPosition> [ <http://ontologydesignpatterns.org/opla-sd#entityPositionX> "-379.54606828843237"^^xsd:double ;
                                                                              <http://ontologydesignpatterns.org/opla-sd#entityPositionY> "259.68463598533674"^^xsd:double ;
                                                                              rdfs:comment "This is an entity positioning annotation generated by CoModIDE (https://comodide.com/). Removing this annotation will break rendering the CoModIDE schema diagram view."@en
                                                                            ] .


###  http://www.w3id.org/dpp/UseAndMaintenance#toolsRequired
:toolsRequired rdf:type owl:DatatypeProperty ;
               rdfs:domain dpp:MaintenanceTask ;
               rdfs:range xsd:string ;
               <http://ontologydesignpatterns.org/opla-sd#entityPosition> [ <http://ontologydesignpatterns.org/opla-sd#entityPositionX> "279.56694122230124"^^xsd:double ;
                                                                            <http://ontologydesignpatterns.org/opla-sd#entityPositionY> "379.76174249670726"^^xsd:double ;
                                                                            rdfs:comment "This is an entity positioning annotation generated by CoModIDE (https://comodide.com/). Removing this annotation will break rendering the CoModIDE schema diagram view."@en
                                                                          ] .


###  http://www.w3id.org/dpp/UseAndMaintenance#useDescription
:useDescription rdf:type owl:DatatypeProperty ;
                rdfs:domain :IntendedUse ;
                rdfs:range xsd:string ;
                <http://ontologydesignpatterns.org/opla-sd#entityPosition> [ <http://ontologydesignpatterns.org/opla-sd#entityPositionX> "810.0175214656736"^^xsd:double ;
                                                                             <http://ontologydesignpatterns.org/opla-sd#entityPositionY> "860.4984330446638"^^xsd:double ;
                                                                             rdfs:comment "This is an entity positioning annotation generated by CoModIDE (https://comodide.com/). Removing this annotation will break rendering the CoModIDE schema diagram view."@en
                                                                           ] ;
                rdfs:comment "textual description of how the product is intended to be used" .


###  http://www.w3id.org/dpp/UseAndMaintenance#useGuidelines
:useGuidelines rdf:type owl:DatatypeProperty ;
               rdfs:domain :IntendedUse ;
               rdfs:range xsd:string ;
               <http://ontologydesignpatterns.org/opla-sd#entityPosition> [ <http://ontologydesignpatterns.org/opla-sd#entityPositionX> "799.7131700359793"^^xsd:double ;
                                                                            <http://ontologydesignpatterns.org/opla-sd#entityPositionY> "759.6982884480636"^^xsd:double ;
                                                                            rdfs:comment "This is an entity positioning annotation generated by CoModIDE (https://comodide.com/). Removing this annotation will break rendering the CoModIDE schema diagram view."@en
                                                                          ] .


###  http://www.w3id.org/dpp/UseAndMaintenance#userID
:userID rdf:type owl:DatatypeProperty ;
        rdfs:domain dpp:User ;
        rdfs:range xsd:string ;
        <http://ontologydesignpatterns.org/opla-sd#entityPosition> [ <http://ontologydesignpatterns.org/opla-sd#entityPositionX> "769.7920528322359"^^xsd:double ;
                                                                     <http://ontologydesignpatterns.org/opla-sd#entityPositionY> "1000.3904080396119"^^xsd:double ;
                                                                     rdfs:comment "This is an entity positioning annotation generated by CoModIDE (https://comodide.com/). Removing this annotation will break rendering the CoModIDE schema diagram view."@en
                                                                   ] .


###  http://www.w3id.org/dpp/UseAndMaintenance#userName
:userName rdf:type owl:DatatypeProperty ;
          rdfs:domain dpp:User ;
          rdfs:range xsd:Name ;
          <http://ontologydesignpatterns.org/opla-sd#entityPosition> [ <http://ontologydesignpatterns.org/opla-sd#entityPositionX> "779.6143700714645"^^xsd:double ;
                                                                       <http://ontologydesignpatterns.org/opla-sd#entityPositionY> "909.637232803242"^^xsd:double ;
                                                                       rdfs:comment "This is an entity positioning annotation generated by CoModIDE (https://comodide.com/). Removing this annotation will break rendering the CoModIDE schema diagram view."@en
                                                                     ] .


###  http://www.w3id.org/dpp/UseAndMaintenance#warrantyID
:warrantyID rdf:type owl:DatatypeProperty ;
            rdfs:domain :Warranty ;
            rdfs:range xsd:string ;
            <http://ontologydesignpatterns.org/opla-sd#entityPosition> [ <http://ontologydesignpatterns.org/opla-sd#entityPositionX> "650.4405266134976"^^xsd:double ;
                                                                         <http://ontologydesignpatterns.org/opla-sd#entityPositionY> "620.1584064486909"^^xsd:double ;
                                                                         rdfs:comment "This is an entity positioning annotation generated by CoModIDE (https://comodide.com/). Removing this annotation will break rendering the CoModIDE schema diagram view."@en
                                                                       ] ;
            rdfs:label "warrantyID" .


###  http://www.w3id.org/dpp/UseAndMaintenance#warrantyPeriod
:warrantyPeriod rdf:type owl:DatatypeProperty ;
                rdfs:domain :Warranty ;
                <http://ontologydesignpatterns.org/opla-sd#entityPosition> [ <http://ontologydesignpatterns.org/opla-sd#entityPositionX> "789.5669412223012"^^xsd:double ;
                                                                             <http://ontologydesignpatterns.org/opla-sd#entityPositionY> "689.7617424967073"^^xsd:double ;
                                                                             rdfs:comment "This is an entity positioning annotation generated by CoModIDE (https://comodide.com/). Removing this annotation will break rendering the CoModIDE schema diagram view."@en
                                                                           ] ;
                rdfs:label "warrantyPeriod" .


#################################################################
#    Classes
#################################################################

###  http://ontologydesignpatterns.org/opla#Module
<http://ontologydesignpatterns.org/opla#Module> rdf:type owl:Class .


###  http://ontologydesignpatterns.org/opla#Pattern
<http://ontologydesignpatterns.org/opla#Pattern> rdf:type owl:Class .


###  http://www.w3id.org/dpp#Activity
dpp:Activity rdf:type owl:Class ;
             <http://ontologydesignpatterns.org/opla-sd#entityPosition> [ <http://ontologydesignpatterns.org/opla-sd#entityPositionX> "450.20777348425247"^^xsd:double ;
                                                                          <http://ontologydesignpatterns.org/opla-sd#entityPositionY> "450.3812582974209"^^xsd:double ;
                                                                          rdfs:comment "This is an entity positioning annotation generated by CoModIDE (https://comodide.com/). Removing this annotation will break rendering the CoModIDE schema diagram view."@en
                                                                        ] ;
             rdfs:comment "Any process or action involved in a Maintenance Task."@en ;
             rdfs:label "Activity"@en .


###  http://www.w3id.org/dpp#Building
dpp:Building rdf:type owl:Class ;
             <http://ontologydesignpatterns.org/opla-sd#entityPosition> [ <http://ontologydesignpatterns.org/opla-sd#entityPositionX> "369.9034683238495"^^xsd:double ;
                                                                          <http://ontologydesignpatterns.org/opla-sd#entityPositionY> "1019.7458805745496"^^xsd:double ;
                                                                          rdfs:comment "This is an entity positioning annotation generated by CoModIDE (https://comodide.com/). Removing this annotation will break rendering the CoModIDE schema diagram view."@en
                                                                        ] ;
             rdfs:comment "A structure where a Product is located."@en ;
             rdfs:label "Building"@en .


###  http://www.w3id.org/dpp#Cleaning
dpp:Cleaning rdf:type owl:Class ;
             <http://ontologydesignpatterns.org/opla-sd#entityPosition> [ <http://ontologydesignpatterns.org/opla-sd#entityPositionX> "30.114152337418474"^^xsd:double ;
                                                                          <http://ontologydesignpatterns.org/opla-sd#entityPositionY> "280.27989584958414"^^xsd:double ;
                                                                          rdfs:comment "This is an entity positioning annotation generated by CoModIDE (https://comodide.com/). Removing this annotation will break rendering the CoModIDE schema diagram view."@en
                                                                        ] ;
             rdfs:comment "Instructions and records related to the cleaning of a Product."@en ;
             rdfs:label "Cleaning"@en .


###  http://www.w3id.org/dpp#Consumable
dpp:Consumable rdf:type owl:Class ;
               <http://ontologydesignpatterns.org/opla-sd#entityPosition> [ <http://ontologydesignpatterns.org/opla-sd#entityPositionX> "29.58440368208494"^^xsd:double ;
                                                                            <http://ontologydesignpatterns.org/opla-sd#entityPositionY> "400.0700960770059"^^xsd:double ;
                                                                            rdfs:comment "This is an entity positioning annotation generated by CoModIDE (https://comodide.com/). Removing this annotation will break rendering the CoModIDE schema diagram view."@en
                                                                          ] ;
               rdfs:comment "Items that are consumed during the use or maintenance of a Product. For example, fuel, etc"@en ;
               rdfs:label "Consumable"@en .


###  http://www.w3id.org/dpp#FailureData
dpp:FailureData rdf:type owl:Class ;
                <http://ontologydesignpatterns.org/opla-sd#entityPosition> [ <http://ontologydesignpatterns.org/opla-sd#entityPositionX> "-139.52853569224231"^^xsd:double ;
                                                                             <http://ontologydesignpatterns.org/opla-sd#entityPositionY> "619.9717881705479"^^xsd:double ;
                                                                             rdfs:comment "This is an entity positioning annotation generated by CoModIDE (https://comodide.com/). Removing this annotation will break rendering the CoModIDE schema diagram view."@en
                                                                           ] ;
                rdfs:comment "Data related to the failure rates of a Product, including mean time between failures."@en ;
                rdfs:label "FailureData"@en .


###  http://www.w3id.org/dpp#MaintenanceRecord
dpp:MaintenanceRecord rdf:type owl:Class ;
                      <http://ontologydesignpatterns.org/opla-sd#entityPosition> [ <http://ontologydesignpatterns.org/opla-sd#entityPositionX> "819.9062618694126"^^xsd:double ;
                                                                                   <http://ontologydesignpatterns.org/opla-sd#entityPositionY> "-339.6987149948836"^^xsd:double ;
                                                                                   rdfs:comment "This is an entity positioning annotation generated by CoModIDE (https://comodide.com/). Removing this annotation will break rendering the CoModIDE schema diagram view."@en
                                                                                 ] ;
                      rdfs:comment "A record of a specific maintenance task, including what was done, who did it, and when."@en ;
                      rdfs:label "MaintenanceRecord"@en .


###  http://www.w3id.org/dpp#MaintenanceTask
dpp:MaintenanceTask rdf:type owl:Class ;
                    rdfs:subClassOf :ProvenanceActivity ;
                    <http://ontologydesignpatterns.org/opla-sd#entityPosition> [ <http://ontologydesignpatterns.org/opla-sd#entityPositionX> "229.7862732656149"^^xsd:double ;
                                                                                 <http://ontologydesignpatterns.org/opla-sd#entityPositionY> "-200.36369276443307"^^xsd:double ;
                                                                                 rdfs:comment "This is an entity positioning annotation generated by CoModIDE (https://comodide.com/). Removing this annotation will break rendering the CoModIDE schema diagram view."@en
                                                                               ] ;
                    rdfs:comment "A scheduled or required action performed to maintain or repair a Product."@en ;
                    rdfs:label "MaintenanceTask"@en .


###  http://www.w3id.org/dpp#MaintenanceTechnician
dpp:MaintenanceTechnician rdf:type owl:Class ;
                          rdfs:subClassOf :AgentRole ;
                          <http://ontologydesignpatterns.org/opla-sd#entityPosition> [ <http://ontologydesignpatterns.org/opla-sd#entityPositionX> "880.1508236685033"^^xsd:double ;
                                                                                       <http://ontologydesignpatterns.org/opla-sd#entityPositionY> "210.00150406144002"^^xsd:double ;
                                                                                       rdfs:comment "This is an entity positioning annotation generated by CoModIDE (https://comodide.com/). Removing this annotation will break rendering the CoModIDE schema diagram view."@en
                                                                                     ] ;
                          rdfs:comment "An individual skilled in performing maintenance tasks."@en ;
                          rdfs:label "MaintenanceTechnician"@en .


###  http://www.w3id.org/dpp#Manual
dpp:Manual rdf:type owl:Class ;
           <http://ontologydesignpatterns.org/opla-sd#entityPosition> [ <http://ontologydesignpatterns.org/opla-sd#entityPositionX> "440.0180560035367"^^xsd:double ;
                                                                        <http://ontologydesignpatterns.org/opla-sd#entityPositionY> "529.8487622450107"^^xsd:double ;
                                                                        rdfs:comment "This is an entity positioning annotation generated by CoModIDE (https://comodide.com/). Removing this annotation will break rendering the CoModIDE schema diagram view."@en
                                                                      ] ;
           rdfs:comment "User manuals, warnings, or safety information related to a Product."@en ;
           rdfs:label "Manual"@en .


###  http://www.w3id.org/dpp#OwnershipStatus
dpp:OwnershipStatus rdf:type owl:Class ;
                    <http://ontologydesignpatterns.org/opla-sd#entityPosition> [ <http://ontologydesignpatterns.org/opla-sd#entityPositionX> "-119.84651102701923"^^xsd:double ;
                                                                                 <http://ontologydesignpatterns.org/opla-sd#entityPositionY> "1059.6554950959444"^^xsd:double ;
                                                                                 rdfs:comment "This is an entity positioning annotation generated by CoModIDE (https://comodide.com/). Removing this annotation will break rendering the CoModIDE schema diagram view."@en
                                                                               ] ;
                    rdfs:comment "Information about the ownership status of a Product."@en ;
                    rdfs:label "OwnershipStatus"@en .


###  http://www.w3id.org/dpp#Product
dpp:Product rdf:type owl:Class ;
            rdfs:subClassOf :EntityWithProvenance ;
            <http://ontologydesignpatterns.org/opla-sd#entityPosition> [ <http://ontologydesignpatterns.org/opla-sd#entityPositionX> "189.9827136371448"^^xsd:double ;
                                                                         <http://ontologydesignpatterns.org/opla-sd#entityPositionY> "840.02689129946"^^xsd:double ;
                                                                         rdfs:comment "This is an entity positioning annotation generated by CoModIDE (https://comodide.com/). Removing this annotation will break rendering the CoModIDE schema diagram view."@en
                                                                       ] .


###  http://www.w3id.org/dpp#RealUseInformation
dpp:RealUseInformation rdf:type owl:Class ;
                       <http://ontologydesignpatterns.org/opla-sd#entityPosition> [ <http://ontologydesignpatterns.org/opla-sd#entityPositionX> "19.61545798835698"^^xsd:double ;
                                                                                    <http://ontologydesignpatterns.org/opla-sd#entityPositionY> "1090.143678273247"^^xsd:double ;
                                                                                    rdfs:comment "This is an entity positioning annotation generated by CoModIDE (https://comodide.com/). Removing this annotation will break rendering the CoModIDE schema diagram view."@en
                                                                                  ] ;
                       rdfs:comment "Information about the actual use conditions and patterns of a Product."@en ;
                       rdfs:label "RealUseInformation"@en .


###  http://www.w3id.org/dpp#ServiceHistory
dpp:ServiceHistory rdf:type owl:Class ;
                   <http://ontologydesignpatterns.org/opla-sd#entityPosition> [ <http://ontologydesignpatterns.org/opla-sd#entityPositionX> "-210.22397890913754"^^xsd:double ;
                                                                                <http://ontologydesignpatterns.org/opla-sd#entityPositionY> "979.989158018367"^^xsd:double ;
                                                                                rdfs:comment "This is an entity positioning annotation generated by CoModIDE (https://comodide.com/). Removing this annotation will break rendering the CoModIDE schema diagram view."@en
                                                                              ] ;
                   rdfs:comment "Records of all maintenance and repair activities performed on a Product."@en ;
                   rdfs:label "ServiceHistory"@en .


###  http://www.w3id.org/dpp#Update
dpp:Update rdf:type owl:Class ;
           <http://ontologydesignpatterns.org/opla-sd#entityPosition> [ <http://ontologydesignpatterns.org/opla-sd#entityPositionX> "-229.60356196472242"^^xsd:double ;
                                                                        <http://ontologydesignpatterns.org/opla-sd#entityPositionY> "890.4985577232903"^^xsd:double ;
                                                                        rdfs:comment "This is an entity positioning annotation generated by CoModIDE (https://comodide.com/). Removing this annotation will break rendering the CoModIDE schema diagram view."@en
                                                                      ] ;
           rdfs:comment "Information about updates made to the Product during its operational phase."@en ;
           rdfs:label "Update"@en .


###  http://www.w3id.org/dpp#UseCondition
dpp:UseCondition rdf:type owl:Class ;
                 <http://ontologydesignpatterns.org/opla-sd#entityPosition> [ <http://ontologydesignpatterns.org/opla-sd#entityPositionX> "599.9186215387032"^^xsd:double ;
                                                                              <http://ontologydesignpatterns.org/opla-sd#entityPositionY> "570.4841283281769"^^xsd:double ;
                                                                              rdfs:comment "This is an entity positioning annotation generated by CoModIDE (https://comodide.com/). Removing this annotation will break rendering the CoModIDE schema diagram view."@en
                                                                            ] ;
                 rdfs:comment "Conditions under which a Product should be used for optimal performance and safety."@en ;
                 rdfs:label "UseCondition"@en .


###  http://www.w3id.org/dpp#User
dpp:User rdf:type owl:Class ;
         rdfs:subClassOf :Agent ;
         <http://ontologydesignpatterns.org/opla-sd#entityPosition> [ <http://ontologydesignpatterns.org/opla-sd#entityPositionX> "470.3111154451776"^^xsd:double ;
                                                                      <http://ontologydesignpatterns.org/opla-sd#entityPositionY> "960.4344792912094"^^xsd:double ;
                                                                      rdfs:comment "This is an entity positioning annotation generated by CoModIDE (https://comodide.com/). Removing this annotation will break rendering the CoModIDE schema diagram view."@en
                                                                    ] ;
         rdfs:comment "An individual or entity that uses the Product."@en ;
         rdfs:label "User"@en .


###  http://www.w3id.org/dpp#Verification
dpp:Verification rdf:type owl:Class ;
                 <http://ontologydesignpatterns.org/opla-sd#entityPosition> [ <http://ontologydesignpatterns.org/opla-sd#entityPositionX> "329.60851902073136"^^xsd:double ;
                                                                              <http://ontologydesignpatterns.org/opla-sd#entityPositionY> "489.86607079155283"^^xsd:double ;
                                                                              rdfs:comment "This is an entity positioning annotation generated by CoModIDE (https://comodide.com/). Removing this annotation will break rendering the CoModIDE schema diagram view."@en
                                                                            ] ;
                 rdfs:comment "Information about verifications made to ensure the Product's integrity and safety."@en ;
                 rdfs:label "Verification"@en .


###  http://www.w3id.org/dpp/UseAndMaintenance#Agent
:Agent rdf:type owl:Class ;
       <http://ontologydesignpatterns.org/opla#isNativeTo> <http://www.w3id.org/dpp/UseAndMaintenance-modules/f5199444-758a-40b7-ad67-4a2a99ee3d2c> ,
                                                           <http://www.w3id.org/dpp/UseAndMaintenance-modules/9892962b-836d-4b8e-b823-bfbc6d2d1e7b> ;
       <http://ontologydesignpatterns.org/opla-sd#entityPosition> [ <http://ontologydesignpatterns.org/opla-sd#entityPositionX> "1139.7473051568222"^^xsd:double ;
                                                                    <http://ontologydesignpatterns.org/opla-sd#entityPositionY> "140.3987275216454"^^xsd:double ;
                                                                    rdfs:comment "This is an entity positioning annotation generated by CoModIDE (https://comodide.com/). Removing this annotation will break rendering the CoModIDE schema diagram view."@en
                                                                  ] .


###  http://www.w3id.org/dpp/UseAndMaintenance#AgentRole
:AgentRole rdf:type owl:Class ;
           <http://ontologydesignpatterns.org/opla#isNativeTo> <http://www.w3id.org/dpp/UseAndMaintenance-modules/f5199444-758a-40b7-ad67-4a2a99ee3d2c> ;
           <http://ontologydesignpatterns.org/opla-sd#entityPosition> [ <http://ontologydesignpatterns.org/opla-sd#entityPositionX> "960.1465844687827"^^xsd:double ;
                                                                        <http://ontologydesignpatterns.org/opla-sd#entityPositionY> "460.04647561629133"^^xsd:double ;
                                                                        rdfs:comment "This is an entity positioning annotation generated by CoModIDE (https://comodide.com/). Removing this annotation will break rendering the CoModIDE schema diagram view."@en
                                                                      ] .


###  http://www.w3id.org/dpp/UseAndMaintenance#ComplexTemporalExtent
:ComplexTemporalExtent rdf:type owl:Class ;
                       <http://ontologydesignpatterns.org/opla#isNativeTo> <http://www.w3id.org/dpp/UseAndMaintenance-modules/35950a21-8fcd-4fbd-a876-e4ec20d5007c> ;
                       <http://ontologydesignpatterns.org/opla-sd#entityPosition> [ <http://ontologydesignpatterns.org/opla-sd#entityPositionX> "1119.9006684392307"^^xsd:double ;
                                                                                    <http://ontologydesignpatterns.org/opla-sd#entityPositionY> "859.6858696623075"^^xsd:double ;
                                                                                    rdfs:comment "This is an entity positioning annotation generated by CoModIDE (https://comodide.com/). Removing this annotation will break rendering the CoModIDE schema diagram view."@en
                                                                                  ] .


###  http://www.w3id.org/dpp/UseAndMaintenance#ContactInformation
:ContactInformation rdf:type owl:Class ;
                    <http://ontologydesignpatterns.org/opla-sd#entityPosition> [ <http://ontologydesignpatterns.org/opla-sd#entityPositionX> "659.9206080002205"^^xsd:double ;
                                                                                 <http://ontologydesignpatterns.org/opla-sd#entityPositionY> "1070.0695144555148"^^xsd:double ;
                                                                                 rdfs:comment "This is an entity positioning annotation generated by CoModIDE (https://comodide.com/). Removing this annotation will break rendering the CoModIDE schema diagram view."@en
                                                                               ] .


###  http://www.w3id.org/dpp/UseAndMaintenance#CostQuantity
:CostQuantity rdf:type owl:Class ;
              rdfs:subClassOf :Quantity ;
              <http://ontologydesignpatterns.org/opla-sd#entityPosition> [ <http://ontologydesignpatterns.org/opla-sd#entityPositionX> "-510.45684302859206"^^xsd:double ;
                                                                           <http://ontologydesignpatterns.org/opla-sd#entityPositionY> "-139.92540945761223"^^xsd:double ;
                                                                           rdfs:comment "This is an entity positioning annotation generated by CoModIDE (https://comodide.com/). Removing this annotation will break rendering the CoModIDE schema diagram view."@en
                                                                         ] ;
              rdfs:comment """hasQuantityKind MaintenanceCost or other cost related activities

hasNumericValue decimal/float value either in USD or SEK ....""" .


###  http://www.w3id.org/dpp/UseAndMaintenance#EntityWithProvenance
:EntityWithProvenance rdf:type owl:Class ;
                      <http://ontologydesignpatterns.org/opla#isNativeTo> <http://www.w3id.org/dpp/UseAndMaintenance-modules/9892962b-836d-4b8e-b823-bfbc6d2d1e7b> ;
                      <http://ontologydesignpatterns.org/opla-sd#entityPosition> [ <http://ontologydesignpatterns.org/opla-sd#entityPositionX> "739.6461703386256"^^xsd:double ;
                                                                                   <http://ontologydesignpatterns.org/opla-sd#entityPositionY> "-129.84375229740618"^^xsd:double ;
                                                                                   rdfs:comment "This is an entity positioning annotation generated by CoModIDE (https://comodide.com/). Removing this annotation will break rendering the CoModIDE schema diagram view."@en
                                                                                 ] .


###  http://www.w3id.org/dpp/UseAndMaintenance#IntendedUse
:IntendedUse rdf:type owl:Class ;
             <http://ontologydesignpatterns.org/opla-sd#entityPosition> [ <http://ontologydesignpatterns.org/opla-sd#entityPositionX> "570.2379536636882"^^xsd:double ;
                                                                          <http://ontologydesignpatterns.org/opla-sd#entityPositionY> "820.1486635044242"^^xsd:double ;
                                                                          rdfs:comment "This is an entity positioning annotation generated by CoModIDE (https://comodide.com/). Removing this annotation will break rendering the CoModIDE schema diagram view."@en
                                                                        ] .


###  http://www.w3id.org/dpp/UseAndMaintenance#Lifespan
:Lifespan rdf:type owl:Class ;
          rdfs:subClassOf :QuantityKind ;
          <http://ontologydesignpatterns.org/opla-sd#entityPosition> [ <http://ontologydesignpatterns.org/opla-sd#entityPositionX> "-69.628143224486"^^xsd:double ;
                                                                       <http://ontologydesignpatterns.org/opla-sd#entityPositionY> "9.699456347320563"^^xsd:double ;
                                                                       rdfs:comment "This is an entity positioning annotation generated by CoModIDE (https://comodide.com/). Removing this annotation will break rendering the CoModIDE schema diagram view."@en
                                                                     ] .


###  http://www.w3id.org/dpp/UseAndMaintenance#LifespanQuantity
:LifespanQuantity rdf:type owl:Class ;
                  rdfs:subClassOf :Quantity ;
                  <http://ontologydesignpatterns.org/opla-sd#entityPosition> [ <http://ontologydesignpatterns.org/opla-sd#entityPositionX> "-799.5825005177697"^^xsd:double ;
                                                                               <http://ontologydesignpatterns.org/opla-sd#entityPositionY> "-10.358393125163673"^^xsd:double ;
                                                                               rdfs:comment "This is an entity positioning annotation generated by CoModIDE (https://comodide.com/). Removing this annotation will break rendering the CoModIDE schema diagram view."@en
                                                                             ] ;
                  rdfs:comment """hasQuantityKind Lifespan

hasNumericValue value in Years (lifespan in years)

If a product has a lifespan of 10 years, set the hasNumericValue of the corresponding QuantityValue instance to 10.""" .


###  http://www.w3id.org/dpp/UseAndMaintenance#MaintenanceCost
:MaintenanceCost rdf:type owl:Class ;
                 rdfs:subClassOf :QuantityKind ;
                 <http://ontologydesignpatterns.org/opla-sd#entityPosition> [ <http://ontologydesignpatterns.org/opla-sd#entityPositionX> "-250.166201330006"^^xsd:double ;
                                                                              <http://ontologydesignpatterns.org/opla-sd#entityPositionY> "-280.0860327216652"^^xsd:double ;
                                                                              rdfs:comment "This is an entity positioning annotation generated by CoModIDE (https://comodide.com/). Removing this annotation will break rendering the CoModIDE schema diagram view."@en
                                                                            ] .


###  http://www.w3id.org/dpp/UseAndMaintenance#MaintenanceSchedule
:MaintenanceSchedule rdf:type owl:Class ;
                     <http://ontologydesignpatterns.org/opla-sd#entityPosition> [ <http://ontologydesignpatterns.org/opla-sd#entityPositionX> "209.94271890682217"^^xsd:double ;
                                                                                  <http://ontologydesignpatterns.org/opla-sd#entityPositionY> "-449.9538005302725"^^xsd:double ;
                                                                                  rdfs:comment "This is an entity positioning annotation generated by CoModIDE (https://comodide.com/). Removing this annotation will break rendering the CoModIDE schema diagram view."@en
                                                                                ] .


###  http://www.w3id.org/dpp/UseAndMaintenance#MaintenanceTeam
:MaintenanceTeam rdf:type owl:Class ;
                 rdfs:subClassOf :Agent ;
                 <http://ontologydesignpatterns.org/opla-sd#entityPosition> [ <http://ontologydesignpatterns.org/opla-sd#entityPositionX> "1219.7780526813644"^^xsd:double ;
                                                                              <http://ontologydesignpatterns.org/opla-sd#entityPositionY> "220.01352254157382"^^xsd:double ;
                                                                              rdfs:comment "This is an entity positioning annotation generated by CoModIDE (https://comodide.com/). Removing this annotation will break rendering the CoModIDE schema diagram view."@en
                                                                            ] .


###  http://www.w3id.org/dpp/UseAndMaintenance#PercentagePerYear
:PercentagePerYear rdf:type owl:Class ;
                   rdfs:subClassOf :Unit ;
                   <http://ontologydesignpatterns.org/opla-sd#entityPosition> [ <http://ontologydesignpatterns.org/opla-sd#entityPositionX> "-379.83118397240804"^^xsd:double ;
                                                                                <http://ontologydesignpatterns.org/opla-sd#entityPositionY> "170.1000184852847"^^xsd:double ;
                                                                                rdfs:comment "This is an entity positioning annotation generated by CoModIDE (https://comodide.com/). Removing this annotation will break rendering the CoModIDE schema diagram view."@en
                                                                              ] ;
                   rdfs:comment "Unit for quantity loss rate measured as a percentage per year" .


###  http://www.w3id.org/dpp/UseAndMaintenance#PointInTime
:PointInTime rdf:type owl:Class ;
             rdfs:subClassOf :ComplexTemporalExtent ;
             <http://ontologydesignpatterns.org/opla#isNativeTo> <http://www.w3id.org/dpp/UseAndMaintenance-modules/35950a21-8fcd-4fbd-a876-e4ec20d5007c> ;
             <http://ontologydesignpatterns.org/opla-sd#entityPosition> [ <http://ontologydesignpatterns.org/opla-sd#entityPositionX> "1260.0883095878094"^^xsd:double ;
                                                                          <http://ontologydesignpatterns.org/opla-sd#entityPositionY> "650.2246202219453"^^xsd:double ;
                                                                          rdfs:comment "This is an entity positioning annotation generated by CoModIDE (https://comodide.com/). Removing this annotation will break rendering the CoModIDE schema diagram view."@en
                                                                        ] .


###  http://www.w3id.org/dpp/UseAndMaintenance#ProvenanceActivity
:ProvenanceActivity rdf:type owl:Class ;
                    <http://ontologydesignpatterns.org/opla#isNativeTo> <http://www.w3id.org/dpp/UseAndMaintenance-modules/9892962b-836d-4b8e-b823-bfbc6d2d1e7b> ;
                    <http://ontologydesignpatterns.org/opla-sd#entityPosition> [ <http://ontologydesignpatterns.org/opla-sd#entityPositionX> "1279.6534420535577"^^xsd:double ;
                                                                                 <http://ontologydesignpatterns.org/opla-sd#entityPositionY> "-210.49897419100995"^^xsd:double ;
                                                                                 rdfs:comment "This is an entity positioning annotation generated by CoModIDE (https://comodide.com/). Removing this annotation will break rendering the CoModIDE schema diagram view."@en
                                                                               ] .


###  http://www.w3id.org/dpp/UseAndMaintenance#QualityLossQuantity
:QualityLossQuantity rdf:type owl:Class ;
                     rdfs:subClassOf :Quantity ;
                     <http://ontologydesignpatterns.org/opla-sd#entityPosition> [ <http://ontologydesignpatterns.org/opla-sd#entityPositionX> "-699.7905687986009"^^xsd:double ;
                                                                                  <http://ontologydesignpatterns.org/opla-sd#entityPositionY> "-69.93670005130971"^^xsd:double ;
                                                                                  rdfs:comment "This is an entity positioning annotation generated by CoModIDE (https://comodide.com/). Removing this annotation will break rendering the CoModIDE schema diagram view."@en
                                                                                ] ;
                     rdfs:comment """hasQuantityKind QualityLossRate over time

hasNumericValue  value in percentagePerYear""" .


###  http://www.w3id.org/dpp/UseAndMaintenance#QualityLossRate
:QualityLossRate rdf:type owl:Class ;
                 rdfs:subClassOf :QuantityKind ;
                 <http://ontologydesignpatterns.org/opla-sd#entityPosition> [ <http://ontologydesignpatterns.org/opla-sd#entityPositionX> "40.02409722035871"^^xsd:double ;
                                                                              <http://ontologydesignpatterns.org/opla-sd#entityPositionY> "-140.17113376143038"^^xsd:double ;
                                                                              rdfs:comment "This is an entity positioning annotation generated by CoModIDE (https://comodide.com/). Removing this annotation will break rendering the CoModIDE schema diagram view."@en
                                                                            ] .


###  http://www.w3id.org/dpp/UseAndMaintenance#Quantity
:Quantity rdf:type owl:Class ;
          <http://ontologydesignpatterns.org/opla#isNativeTo> <http://www.w3id.org/dpp/UseAndMaintenance-modules/3688421d-d7b1-45c5-b117-5cfe3320ffd4> ;
          <http://ontologydesignpatterns.org/opla-sd#entityPosition> [ <http://ontologydesignpatterns.org/opla-sd#entityPositionX> "-519.7525483346735"^^xsd:double ;
                                                                       <http://ontologydesignpatterns.org/opla-sd#entityPositionY> "10.20215781171072"^^xsd:double ;
                                                                       rdfs:comment "This is an entity positioning annotation generated by CoModIDE (https://comodide.com/). Removing this annotation will break rendering the CoModIDE schema diagram view."@en
                                                                     ] .


###  http://www.w3id.org/dpp/UseAndMaintenance#QuantityKind
:QuantityKind rdf:type owl:Class ;
              <http://ontologydesignpatterns.org/opla#isNativeTo> <http://www.w3id.org/dpp/UseAndMaintenance-modules/3688421d-d7b1-45c5-b117-5cfe3320ffd4> ;
              <http://ontologydesignpatterns.org/opla-sd#entityPosition> [ <http://ontologydesignpatterns.org/opla-sd#entityPositionX> "-320.36328028277296"^^xsd:double ;
                                                                           <http://ontologydesignpatterns.org/opla-sd#entityPositionY> "-59.77605585233971"^^xsd:double ;
                                                                           rdfs:comment "This is an entity positioning annotation generated by CoModIDE (https://comodide.com/). Removing this annotation will break rendering the CoModIDE schema diagram view."@en
                                                                         ] .


###  http://www.w3id.org/dpp/UseAndMaintenance#QuantityValue
:QuantityValue rdf:type owl:Class ;
               <http://ontologydesignpatterns.org/opla#isNativeTo> <http://www.w3id.org/dpp/UseAndMaintenance-modules/3688421d-d7b1-45c5-b117-5cfe3320ffd4> ;
               <http://ontologydesignpatterns.org/opla-sd#entityPosition> [ <http://ontologydesignpatterns.org/opla-sd#entityPositionX> "-540.4823538796089"^^xsd:double ;
                                                                            <http://ontologydesignpatterns.org/opla-sd#entityPositionY> "160.14059370729905"^^xsd:double ;
                                                                            rdfs:comment "This is an entity positioning annotation generated by CoModIDE (https://comodide.com/). Removing this annotation will break rendering the CoModIDE schema diagram view."@en
                                                                          ] .


###  http://www.w3id.org/dpp/UseAndMaintenance#ReferenceSystem
:ReferenceSystem rdf:type owl:Class ;
                 <http://ontologydesignpatterns.org/opla#isNativeTo> <http://www.w3id.org/dpp/UseAndMaintenance-modules/35950a21-8fcd-4fbd-a876-e4ec20d5007c> ;
                 <http://ontologydesignpatterns.org/opla-sd#entityPosition> [ <http://ontologydesignpatterns.org/opla-sd#entityPositionX> "1380.401137192358"^^xsd:double ;
                                                                              <http://ontologydesignpatterns.org/opla-sd#entityPositionY> "979.8768357316287"^^xsd:double ;
                                                                              rdfs:comment "This is an entity positioning annotation generated by CoModIDE (https://comodide.com/). Removing this annotation will break rendering the CoModIDE schema diagram view."@en
                                                                            ] .


###  http://www.w3id.org/dpp/UseAndMaintenance#SEK
:SEK rdf:type owl:Class ;
     rdfs:subClassOf :Unit .


###  http://www.w3id.org/dpp/UseAndMaintenance#SafetyMeasure
:SafetyMeasure rdf:type owl:Class ;
               <http://ontologydesignpatterns.org/opla-sd#entityPosition> [ <http://ontologydesignpatterns.org/opla-sd#entityPositionX> "900.304217085686"^^xsd:double ;
                                                                            <http://ontologydesignpatterns.org/opla-sd#entityPositionY> "-250.40355247499497"^^xsd:double ;
                                                                            rdfs:comment "This is an entity positioning annotation generated by CoModIDE (https://comodide.com/). Removing this annotation will break rendering the CoModIDE schema diagram view."@en
                                                                          ] .


###  http://www.w3id.org/dpp/UseAndMaintenance#TemporalExtent
:TemporalExtent rdf:type owl:Class ;
                <http://ontologydesignpatterns.org/opla#isNativeTo> <http://www.w3id.org/dpp/UseAndMaintenance-modules/f5199444-758a-40b7-ad67-4a2a99ee3d2c> ,
                                                                    <http://www.w3id.org/dpp/UseAndMaintenance-modules/35950a21-8fcd-4fbd-a876-e4ec20d5007c> ;
                <http://ontologydesignpatterns.org/opla-sd#entityPosition> [ <http://ontologydesignpatterns.org/opla-sd#entityPositionX> "1159.8115692753297"^^xsd:double ;
                                                                             <http://ontologydesignpatterns.org/opla-sd#entityPositionY> "560.3884127798827"^^xsd:double ;
                                                                             rdfs:comment "This is an entity positioning annotation generated by CoModIDE (https://comodide.com/). Removing this annotation will break rendering the CoModIDE schema diagram view."@en
                                                                           ] .


###  http://www.w3id.org/dpp/UseAndMaintenance#TimeInterval
:TimeInterval rdf:type owl:Class ;
              rdfs:subClassOf :ComplexTemporalExtent ;
              <http://ontologydesignpatterns.org/opla#isNativeTo> <http://www.w3id.org/dpp/UseAndMaintenance-modules/35950a21-8fcd-4fbd-a876-e4ec20d5007c> ;
              <http://ontologydesignpatterns.org/opla-sd#entityPosition> [ <http://ontologydesignpatterns.org/opla-sd#entityPositionX> "900.0048825899992"^^xsd:double ;
                                                                           <http://ontologydesignpatterns.org/opla-sd#entityPositionY> "730.277472641532"^^xsd:double ;
                                                                           rdfs:comment "This is an entity positioning annotation generated by CoModIDE (https://comodide.com/). Removing this annotation will break rendering the CoModIDE schema diagram view."@en
                                                                         ] .


###  http://www.w3id.org/dpp/UseAndMaintenance#USD
:USD rdf:type owl:Class ;
     rdfs:subClassOf :Unit .


###  http://www.w3id.org/dpp/UseAndMaintenance#Unit
:Unit rdf:type owl:Class ;
      <http://ontologydesignpatterns.org/opla#isNativeTo> <http://www.w3id.org/dpp/UseAndMaintenance-modules/3688421d-d7b1-45c5-b117-5cfe3320ffd4> ;
      <http://ontologydesignpatterns.org/opla-sd#entityPosition> [ <http://ontologydesignpatterns.org/opla-sd#entityPositionX> "-340.1769035504625"^^xsd:double ;
                                                                   <http://ontologydesignpatterns.org/opla-sd#entityPositionY> "90.12565484859402"^^xsd:double ;
                                                                   rdfs:comment "This is an entity positioning annotation generated by CoModIDE (https://comodide.com/). Removing this annotation will break rendering the CoModIDE schema diagram view."@en
                                                                 ] .


###  http://www.w3id.org/dpp/UseAndMaintenance#Value
:Value rdf:type owl:Class ;
       <http://ontologydesignpatterns.org/opla#isNativeTo> <http://www.w3id.org/dpp/UseAndMaintenance-modules/35950a21-8fcd-4fbd-a876-e4ec20d5007c> ;
       <http://ontologydesignpatterns.org/opla-sd#entityPosition> [ <http://ontologydesignpatterns.org/opla-sd#entityPositionX> "1319.5496841371391"^^xsd:double ;
                                                                    <http://ontologydesignpatterns.org/opla-sd#entityPositionY> "539.9011347429973"^^xsd:double ;
                                                                    rdfs:comment "This is an entity positioning annotation generated by CoModIDE (https://comodide.com/). Removing this annotation will break rendering the CoModIDE schema diagram view."@en
                                                                  ] .


###  http://www.w3id.org/dpp/UseAndMaintenance#Warranty
:Warranty rdf:type owl:Class ;
          <http://ontologydesignpatterns.org/opla-sd#entityPosition> [ <http://ontologydesignpatterns.org/opla-sd#entityPositionX> "659.8619229431249"^^xsd:double ;
                                                                       <http://ontologydesignpatterns.org/opla-sd#entityPositionY> "729.649485074669"^^xsd:double ;
                                                                       rdfs:comment "This is an entity positioning annotation generated by CoModIDE (https://comodide.com/). Removing this annotation will break rendering the CoModIDE schema diagram view."@en
                                                                     ] .


###  http://www.w3id.org/dpp/UseAndMaintenance#Years
:Years rdf:type owl:Class ;
       rdfs:subClassOf :Unit .


#################################################################
#    Individuals
#################################################################

###  http://www.w3id.org/dpp/UseAndMaintenance#SEK
:SEK rdf:type owl:NamedIndividual ,
              :SEK .


###  http://www.w3id.org/dpp/UseAndMaintenance#USD
:USD rdf:type owl:NamedIndividual ,
              :USD .


###  http://www.w3id.org/dpp/UseAndMaintenance#Years
:Years rdf:type owl:NamedIndividual ,
                :Years .


###  http://www.w3id.org/dpp/UseAndMaintenance#annualMaintenanceCost
:annualMaintenanceCost rdf:type owl:NamedIndividual ,
                                :MaintenanceCost .


###  http://www.w3id.org/dpp/UseAndMaintenance#percentagePerYear
:percentagePerYear rdf:type owl:NamedIndividual ,
                            :PercentagePerYear .


###  http://www.w3id.org/dpp/UseAndMaintenance-modules/e69a1c0c-bdf8-472b-8b5f-6cf8952bd8df
<http://www.w3id.org/dpp/UseAndMaintenance-modules/e69a1c0c-bdf8-472b-8b5f-6cf8952bd8df> rdf:type owl:NamedIndividual ,
                                                                                                  <http://ontologydesignpatterns.org/opla#Module> ;
                                                                                         <http://ontologydesignpatterns.org/opla#reusesPatternAsTemplate> <https://archive.org/services/purl/domain/modular_ontology_design_library/spatialextent> ;
                                                                                         rdfs:label "'Spatial Extent' ODP Instantiation Module" .


###  http://www.w3id.org/dpp/UseAndMaintenance-modules/f5199444-758a-40b7-ad67-4a2a99ee3d2c
<http://www.w3id.org/dpp/UseAndMaintenance-modules/f5199444-758a-40b7-ad67-4a2a99ee3d2c> rdf:type owl:NamedIndividual ,
                                                                                                  <http://ontologydesignpatterns.org/opla#Module> ;
                                                                                         <http://ontologydesignpatterns.org/opla#reusesPatternAsTemplate> <https://archive.org/services/purl/domain/modular_ontology_design_library/agentrole> ;
                                                                                         rdfs:label "'Agent Role' ODP Instantiation Module" .


###  http://www.w3id.org/dpp/UseAndMaintenance-modules/35950a21-8fcd-4fbd-a876-e4ec20d5007c
<http://www.w3id.org/dpp/UseAndMaintenance-modules/35950a21-8fcd-4fbd-a876-e4ec20d5007c> rdf:type owl:NamedIndividual ,
                                                                                                  <http://ontologydesignpatterns.org/opla#Module> ;
                                                                                         <http://ontologydesignpatterns.org/opla#reusesPatternAsTemplate> <https://archive.org/services/purl/domain/modular_ontology_design_library/temporalextent> ;
                                                                                         rdfs:label "'Temporal Extent' ODP Instantiation Module" .


###  http://www.w3id.org/dpp/UseAndMaintenance-modules/3688421d-d7b1-45c5-b117-5cfe3320ffd4
<http://www.w3id.org/dpp/UseAndMaintenance-modules/3688421d-d7b1-45c5-b117-5cfe3320ffd4> rdf:type owl:NamedIndividual ,
                                                                                                  <http://ontologydesignpatterns.org/opla#Module> ;
                                                                                         <http://ontologydesignpatterns.org/opla#reusesPatternAsTemplate> <https://archive.org/services/purl/domain/modular_ontology_design_library/quantity> ;
                                                                                         rdfs:label "'Quantities and Units' ODP Instantiation Module" .


###  http://www.w3id.org/dpp/UseAndMaintenance-modules/9892962b-836d-4b8e-b823-bfbc6d2d1e7b
<http://www.w3id.org/dpp/UseAndMaintenance-modules/9892962b-836d-4b8e-b823-bfbc6d2d1e7b> rdf:type owl:NamedIndividual ,
                                                                                                  <http://ontologydesignpatterns.org/opla#Module> ;
                                                                                         <http://ontologydesignpatterns.org/opla#reusesPatternAsTemplate> <https://archive.org/services/purl/domain/modular_ontology_design_library/provenance> ;
                                                                                         rdfs:label "'Provenance' ODP Instantiation Module" .


###  https://archive.org/services/purl/domain/modular_ontology_design_library/agentrole
<https://archive.org/services/purl/domain/modular_ontology_design_library/agentrole> rdf:type owl:NamedIndividual ,
                                                                                              <http://ontologydesignpatterns.org/opla#Pattern> ;
                                                                                     rdfs:label "Agent Role" .


###  https://archive.org/services/purl/domain/modular_ontology_design_library/provenance
<https://archive.org/services/purl/domain/modular_ontology_design_library/provenance> rdf:type owl:NamedIndividual ,
                                                                                               <http://ontologydesignpatterns.org/opla#Pattern> ;
                                                                                      rdfs:label "Provenance" .


###  https://archive.org/services/purl/domain/modular_ontology_design_library/quantity
<https://archive.org/services/purl/domain/modular_ontology_design_library/quantity> rdf:type owl:NamedIndividual ,
                                                                                             <http://ontologydesignpatterns.org/opla#Pattern> ;
                                                                                    rdfs:label "Quantities and Units" .


###  https://archive.org/services/purl/domain/modular_ontology_design_library/spatialextent
<https://archive.org/services/purl/domain/modular_ontology_design_library/spatialextent> rdf:type owl:NamedIndividual ,
                                                                                                  <http://ontologydesignpatterns.org/opla#Pattern> ;
                                                                                         rdfs:label "Spatial Extent" .


###  https://archive.org/services/purl/domain/modular_ontology_design_library/temporalextent
<https://archive.org/services/purl/domain/modular_ontology_design_library/temporalextent> rdf:type owl:NamedIndividual ,
                                                                                                   <http://ontologydesignpatterns.org/opla#Pattern> ;
                                                                                          rdfs:label "Temporal Extent" .


[ <http://ontologydesignpatterns.org/opla-sd#entityPositionX> "-159.57558846376932"^^xsd:double ;
  <http://ontologydesignpatterns.org/opla-sd#entityPositionY> "540.323837492171"^^xsd:double ;
  rdfs:comment "This is an entity positioning annotation generated by CoModIDE (https://comodide.com/). Removing this annotation will break rendering the CoModIDE schema diagram view."@en
] .

[ <http://ontologydesignpatterns.org/opla-sd#entityPositionX> "1064.0243776402094"^^xsd:double ;
   <http://ontologydesignpatterns.org/opla-sd#entityPositionY> "880.0231488254697"^^xsd:double ;
   rdfs:comment "This is an entity positioning annotation generated by CoModIDE (https://comodide.com/). Removing this annotation will break rendering the CoModIDE schema diagram view."@en
 ] .

[ <http://ontologydesignpatterns.org/opla-sd#entityPositionX> "1360.4429095432372"^^xsd:double ;
   <http://ontologydesignpatterns.org/opla-sd#entityPositionY> "-89.99168291599509"^^xsd:double ;
   rdfs:comment "This is an entity positioning annotation generated by CoModIDE (https://comodide.com/). Removing this annotation will break rendering the CoModIDE schema diagram view."@en
 ] .

[ <http://ontologydesignpatterns.org/opla-sd#entityPositionX> "-150.3589190153328"^^xsd:double ;
   <http://ontologydesignpatterns.org/opla-sd#entityPositionY> "-239.8515738377631"^^xsd:double ;
   rdfs:comment "This is an entity positioning annotation generated by CoModIDE (https://comodide.com/). Removing this annotation will break rendering the CoModIDE schema diagram view."@en
 ] .

[ <http://ontologydesignpatterns.org/opla-sd#entityPositionX> "1579.891225649416"^^xsd:double ;
   <http://ontologydesignpatterns.org/opla-sd#entityPositionY> "1040.2057304344266"^^xsd:double ;
   rdfs:comment "This is an entity positioning annotation generated by CoModIDE (https://comodide.com/). Removing this annotation will break rendering the CoModIDE schema diagram view."@en
 ] .

[ <http://ontologydesignpatterns.org/opla-sd#entityPositionX> "1263.8789039752776"^^xsd:double ;
   <http://ontologydesignpatterns.org/opla-sd#entityPositionY> "1030.336851876469"^^xsd:double ;
   rdfs:comment "This is an entity positioning annotation generated by CoModIDE (https://comodide.com/). Removing this annotation will break rendering the CoModIDE schema diagram view."@en
 ] .

[ <http://ontologydesignpatterns.org/opla-sd#entityPositionX> "1109.542628027093"^^xsd:double ;
   <http://ontologydesignpatterns.org/opla-sd#entityPositionY> "830.3694557070859"^^xsd:double ;
   rdfs:comment "This is an entity positioning annotation generated by CoModIDE (https://comodide.com/). Removing this annotation will break rendering the CoModIDE schema diagram view."@en
 ] .

[ <http://ontologydesignpatterns.org/opla-sd#entityPositionX> "1459.825237333302"^^xsd:double ;
   <http://ontologydesignpatterns.org/opla-sd#entityPositionY> "950.3479326586407"^^xsd:double ;
   rdfs:comment "This is an entity positioning annotation generated by CoModIDE (https://comodide.com/). Removing this annotation will break rendering the CoModIDE schema diagram view."@en
 ] .

[ <http://ontologydesignpatterns.org/opla-sd#entityPositionX> "1319.8260368693464"^^xsd:double ;
   <http://ontologydesignpatterns.org/opla-sd#entityPositionY> "1050.1444261404577"^^xsd:double ;
   rdfs:comment "This is an entity positioning annotation generated by CoModIDE (https://comodide.com/). Removing this annotation will break rendering the CoModIDE schema diagram view."@en
 ] .

[ <http://ontologydesignpatterns.org/opla-sd#entityPositionX> "1053.9047624902255"^^xsd:double ;
   <http://ontologydesignpatterns.org/opla-sd#entityPositionY> "949.8340314495616"^^xsd:double ;
   rdfs:comment "This is an entity positioning annotation generated by CoModIDE (https://comodide.com/). Removing this annotation will break rendering the CoModIDE schema diagram view."@en
 ] .

[ <http://ontologydesignpatterns.org/opla-sd#entityPositionX> "1054.4801480916099"^^xsd:double ;
   <http://ontologydesignpatterns.org/opla-sd#entityPositionY> "1030.24125198784"^^xsd:double ;
   rdfs:comment "This is an entity positioning annotation generated by CoModIDE (https://comodide.com/). Removing this annotation will break rendering the CoModIDE schema diagram view."@en
 ] .

[ <http://ontologydesignpatterns.org/opla-sd#entityPositionX> "1053.6084475113998"^^xsd:double ;
   <http://ontologydesignpatterns.org/opla-sd#entityPositionY> "1130.3158172726392"^^xsd:double ;
   rdfs:comment "This is an entity positioning annotation generated by CoModIDE (https://comodide.com/). Removing this annotation will break rendering the CoModIDE schema diagram view."@en
 ] .

[ <http://ontologydesignpatterns.org/opla-sd#entityPositionX> "879.6623862033723"^^xsd:double ;
   <http://ontologydesignpatterns.org/opla-sd#entityPositionY> "791.5215945644288"^^xsd:double ;
   rdfs:comment "This is an entity positioning annotation generated by CoModIDE (https://comodide.com/). Removing this annotation will break rendering the CoModIDE schema diagram view."@en
 ] .

[ <http://ontologydesignpatterns.org/opla-sd#entityPositionX> "1460.0136757208757"^^xsd:double ;
   <http://ontologydesignpatterns.org/opla-sd#entityPositionY> "840.0863175912465"^^xsd:double ;
   rdfs:comment "This is an entity positioning annotation generated by CoModIDE (https://comodide.com/). Removing this annotation will break rendering the CoModIDE schema diagram view."@en
 ] .

[ <http://ontologydesignpatterns.org/opla-sd#entityPositionX> "-49.9917222612257"^^xsd:double ;
   <http://ontologydesignpatterns.org/opla-sd#entityPositionY> "9.94781944598222"^^xsd:double ;
   rdfs:comment "This is an entity positioning annotation generated by CoModIDE (https://comodide.com/). Removing this annotation will break rendering the CoModIDE schema diagram view."@en
 ] .

[ <http://ontologydesignpatterns.org/opla-sd#entityPositionX> "1195.7296936046193"^^xsd:double ;
   <http://ontologydesignpatterns.org/opla-sd#entityPositionY> "570.8089695942897"^^xsd:double ;
   rdfs:comment "This is an entity positioning annotation generated by CoModIDE (https://comodide.com/). Removing this annotation will break rendering the CoModIDE schema diagram view."@en
 ] .

[ <http://ontologydesignpatterns.org/opla-sd#entityPositionX> "1063.976982335805"^^xsd:double ;
   <http://ontologydesignpatterns.org/opla-sd#entityPositionY> "759.6590448221539"^^xsd:double ;
   rdfs:comment "This is an entity positioning annotation generated by CoModIDE (https://comodide.com/). Removing this annotation will break rendering the CoModIDE schema diagram view."@en
 ] .

[ <http://ontologydesignpatterns.org/opla-sd#entityPositionX> "248.17248465091012"^^xsd:double ;
   <http://ontologydesignpatterns.org/opla-sd#entityPositionY> "142.06015192774674"^^xsd:double ;
   rdfs:comment "This is an entity positioning annotation generated by CoModIDE (https://comodide.com/). Removing this annotation will break rendering the CoModIDE schema diagram view."@en
 ] .

[ <http://ontologydesignpatterns.org/opla-sd#entityPositionX> "1174.64175432983"^^xsd:double ;
   <http://ontologydesignpatterns.org/opla-sd#entityPositionY> "621.4824502523768"^^xsd:double ;
   rdfs:comment "This is an entity positioning annotation generated by CoModIDE (https://comodide.com/). Removing this annotation will break rendering the CoModIDE schema diagram view."@en
 ] .

[ <http://ontologydesignpatterns.org/opla-sd#entityPositionX> "1225.8351336810003"^^xsd:double ;
   <http://ontologydesignpatterns.org/opla-sd#entityPositionY> "750.7818165698634"^^xsd:double ;
   rdfs:comment "This is an entity positioning annotation generated by CoModIDE (https://comodide.com/). Removing this annotation will break rendering the CoModIDE schema diagram view."@en
 ] .

[ <http://ontologydesignpatterns.org/opla-sd#entityPositionX> "1283.3005560015401"^^xsd:double ;
   <http://ontologydesignpatterns.org/opla-sd#entityPositionY> "503.3688570025008"^^xsd:double ;
   rdfs:comment "This is an entity positioning annotation generated by CoModIDE (https://comodide.com/). Removing this annotation will break rendering the CoModIDE schema diagram view."@en
 ] .

[ <http://ontologydesignpatterns.org/opla-sd#entityPositionX> "48.56694122230127"^^xsd:double ;
   <http://ontologydesignpatterns.org/opla-sd#entityPositionY> "173.76174249670726"^^xsd:double ;
   rdfs:comment "This is an entity positioning annotation generated by CoModIDE (https://comodide.com/). Removing this annotation will break rendering the CoModIDE schema diagram view."@en
 ] .

[ <http://ontologydesignpatterns.org/opla-sd#entityPositionX> "1280.281264702889"^^xsd:double ;
   <http://ontologydesignpatterns.org/opla-sd#entityPositionY> "889.5891149601008"^^xsd:double ;
   rdfs:comment "This is an entity positioning annotation generated by CoModIDE (https://comodide.com/). Removing this annotation will break rendering the CoModIDE schema diagram view."@en
 ] .

[ <http://ontologydesignpatterns.org/opla-sd#entityPositionX> "1573.989330796225"^^xsd:double ;
   <http://ontologydesignpatterns.org/opla-sd#entityPositionY> "-188.60892669253658"^^xsd:double ;
   rdfs:comment "This is an entity positioning annotation generated by CoModIDE (https://comodide.com/). Removing this annotation will break rendering the CoModIDE schema diagram view."@en
 ] .

[ <http://ontologydesignpatterns.org/opla-sd#entityPositionX> "1580.6036686809932"^^xsd:double ;
   <http://ontologydesignpatterns.org/opla-sd#entityPositionY> "-13.374258097809275"^^xsd:double ;
   rdfs:comment "This is an entity positioning annotation generated by CoModIDE (https://comodide.com/). Removing this annotation will break rendering the CoModIDE schema diagram view."@en
 ] .

#################################################################
#    Annotations
#################################################################

:SEK <http://ontologydesignpatterns.org/opla-sd#entityPosition> [ <http://ontologydesignpatterns.org/opla-sd#entityPositionX> "-299.53340714259366"^^xsd:double ;
                                                                   <http://ontologydesignpatterns.org/opla-sd#entityPositionY> "39.99846156226789"^^xsd:double ;
                                                                   rdfs:comment "This is an entity positioning annotation generated by CoModIDE (https://comodide.com/). Removing this annotation will break rendering the CoModIDE schema diagram view."@en
                                                                 ] .


:USD <http://ontologydesignpatterns.org/opla-sd#entityPosition> [ <http://ontologydesignpatterns.org/opla-sd#entityPositionX> "-279.8903226160787"^^xsd:double ;
                                                                  <http://ontologydesignpatterns.org/opla-sd#entityPositionY> "249.5003961834319"^^xsd:double ;
                                                                  rdfs:comment "This is an entity positioning annotation generated by CoModIDE (https://comodide.com/). Removing this annotation will break rendering the CoModIDE schema diagram view."@en
                                                                ] .


:Years <http://ontologydesignpatterns.org/opla-sd#entityPosition> [ <http://ontologydesignpatterns.org/opla-sd#entityPositionX> "-100.02274742855587"^^xsd:double ;
                                                                    <http://ontologydesignpatterns.org/opla-sd#entityPositionY> "139.94412996761514"^^xsd:double ;
                                                                    rdfs:comment "This is an entity positioning annotation generated by CoModIDE (https://comodide.com/). Removing this annotation will break rendering the CoModIDE schema diagram view."@en
                                                                  ] ;
       rdfs:comment "Unit for Lifespan" .


###  Generated by the OWL API (version 4.5.26.2023-07-17T20:34:13Z) https://github.com/owlcs/owlapi
